NBE.lean
@@ -2,4 +2,4 @@
 -- Import modules here that should be built as part of the library.
 import NBE.Kripke
 import NBE.SingleSortBeta
-import NBE.SingleSortBeta
+import NBE.SingleSortBetaEta
